Switch to new def. of wellformedness
We make the new definition of wellformedness introduced recently the
default, though we also keep the old definition (and a proof of its
equivalence) around.

The main benefit of this is a lot of deleted code related to the old
definition, including a rather nasty proof that substitution preserves
wellformedness. This property, and some others, are now proven more
easily. Besides, the new definition allows for simpler automation.

src/WfAlt.v
@@ -1,14 +1,141 @@
-Require Import Contractive Env Free FreeFacts Msg Shape Sty Tac Var Wf.
+Require Import Contractive ContractiveFacts Env Free FreeFacts Msg Shape Sty
+  Tac Var Wf.
 
-Definition wellformed' (S : Sty) := Contractive S /\ Closed S.
+Inductive ok : Env -> Sty -> Prop :=
+| ok_end :
+    forall xs, ok xs unit
+| ok_send :
+    forall xs msg ty,
+    checked xs ty ->
+    ok xs (send msg ty)
+| ok_recv :
+    forall xs msg ty,
+    checked xs ty ->
+    ok xs (recv msg ty)
+| ok_ichoice :
+    forall xs ty1 ty2,
+    checked xs ty1 ->
+    checked xs ty2 ->
+    ok xs (ichoice ty1 ty2)
+| ok_echoice :
+    forall xs ty1 ty2,
+    checked xs ty1 ->
+    checked xs ty2 ->
+    ok xs (echoice ty1 ty2)
+| ok_mu :
+    forall x xs ty,
+    ok (env_add x xs) ty ->
+    ok xs (mu x ty)
+with
+  checked : Env -> Sty -> Prop :=
+  | checked_var :
+      forall x xs,
+      env_mem x xs ->
+      checked xs (var x)
+  | checked_ok :
+      forall xs ty,
+      ok xs ty ->
+      checked xs ty
+.
+Hint Constructors ok : wf.
+Hint Constructors checked : wf.
+
+Scheme ok_ind_mut := Induction for ok Sort Prop
+with checked_ind_mut := Induction for checked Sort Prop.
+
+Definition wellformed' S := ok env_empty S.
 
 
-Lemma wellformed_wellformed' :
+Lemma ok_checked_Contractive :
   forall S,
-  wellformed S -> wellformed' S.
+  (forall XS, ok XS S -> Contractive S) /\
+  (forall XS, checked XS S -> Contractive S).
+Proof.
+  induction S; split; introv H; try (decompose_and IHS); constructor; inverts1 H;
+    repeat match goal with
+    | H : checked _ _ |- _ => inverts H
+    end; try solve
+    [constructor | eauto 3 | inverts H; eauto].
+  - inverts H; simpl; autodiscriminate.
+  - inverts2 H; simpl; autodiscriminate.
+Qed.
+
+Lemma ok_Contractive :
+  forall S XS,
+  ok XS S ->
+  Contractive S.
+Proof. introv H. pose proof (ok_checked_Contractive S). jauto. Qed.
+
+Lemma checked_Contractive :
+  forall S XS,
+  checked XS S ->
+  Contractive S.
+Proof. introv H. pose proof (ok_checked_Contractive S). jauto. Qed.
+
+Lemma wellformed'_Contractive :
+  forall S,
+  wellformed' S ->
+  Contractive S.
+Proof. unfold wellformed'. intros. eauto using ok_Contractive. Qed.
+
+
+Lemma ok_checked_free :
+  forall S X XS,
+  ok XS S \/ checked XS S ->
+  ~ env_mem X XS ->
+  ~ Free X S.
+Proof.
+  induction S; introv Hok Henv; decompose_or_auto;
+    auto with free;
+    match goal with
+    | |- context [var _]     => idtac
+    | Hok : ok _ _      |- _ => inverts1 Hok
+    | Hok : checked _ _ |- _ => inverts2 Hok
+    end; eauto 6 with free.
+
+    introv H; inverts H; eapply IHS; eauto with free;
+    introv H; apply env_mem_add in H; auto.
+
+    introv H; inverts H; eapply IHS; eauto with free;
+    introv H; apply env_mem_add in H; auto.
+
+    inverts1 Hok.
+
+    inverts1 Hok.
+      introv H. inverts1 H. auto.
+      inverts Hok.
+Qed.
+
+
+Lemma ok_free :
+  forall S X XS,
+  ok XS S ->
+  ~ env_mem X XS ->
+  ~ Free X S.
+Proof. intros. eapply ok_checked_free; eauto. Qed.
+
+
+Lemma checked_free :
+  forall S X XS,
+  checked XS S ->
+  ~ env_mem X XS ->
+  ~ Free X S.
+Proof. intros. eapply ok_checked_free; eauto. Qed.
+
+
+Lemma wellformed'_closed : forall S, wellformed' S -> Closed S.
+Proof.
+  unfold wellformed'. unfold Closed. intros S Hwf X. eapply ok_free;
+    eauto with env.
+Qed.
+
+
+Lemma wellformed'_wellformed :
+  forall S,
+  wellformed' S -> wellformed S.
 Proof.
   introv H. unfolds. split;
-  auto using wellformed_Contractive, wellformed_closed.
+  auto using wellformed'_Contractive, wellformed'_closed.
 Qed.
 
 
@@ -40,9 +167,9 @@ Proof.
 Qed.
 
 
-Lemma wellformed'_wellformed :
+Lemma wellformed_wellformed' :
   forall S,
-  wellformed' S -> wellformed S.
+  wellformed S -> wellformed' S.
 Proof.
   introv H. inversion H as [Hcontractive Hclosed].
   apply free_contractive_checked_ok.
