src/ContractiveFacts.v
@@ -1,0 +1,25 @@
+Require Import Contractive Sty Shape.
+
+(******************************************************************************)
+(* Automation *)
+
+
+Hint Extern 2 (Contractive ?S) =>
+  let inv H := solve [inversion H; assumption] in
+  match goal with
+  | H : Contractive (send _ S) |- _ => inv H
+  | H : Contractive (recv _ S) |- _ => inv H
+  | H : Contractive (echoice S _) |- _ => inv H
+  | H : Contractive (echoice _ S) |- _ => inv H
+  | H : Contractive (ichoice S _) |- _ => inv H
+  | H : Contractive (ichoice _ S) |- _ => inv H
+  | H : Contractive (mu _ S) |- _ => inv H
+  end
+: contractive.
+
+
+Hint Extern 2 (shape ?S <> varS) =>
+  match goal with
+  | H : Contractive (mu _ S) |- _ => solve [inversion H; assumption]
+  end
+: contractive.
