src/TraceBisimEquiv.v
@@ -1,113 +1,73 @@
 Require Import Contractive CS CSFacts Equiv Free Sty Subst SubstFacts Msg Tac
-  TL TLFacts Var Wf.
+  TL TLFacts Var Wf WfFacts.
 
 
 Create HintDb tleq discriminated.
 
 
-Inductive R_trace_equality_equivalence : Sty -> Sty -> Prop :=
-| R_trace_equality_equivalence_intro :
-    forall S S' eta (Swf : wellformed S) (S'wf : wellformed S'),
-    tl eta S (wellformed_Contractive S Swf) =
-      tl eta S' (wellformed_Contractive S' S'wf) ->
-    R_trace_equality_equivalence S S'.
-Hint Constructors R_trace_equality_equivalence : tleq.
+Inductive R_trace_bisim_equivalence' : Sty -> Sty -> Prop :=
+| R_trace_bisim_equivalence'_intro :
+    forall S S' eta c c',
+    wellformed S ->
+    wellformed S' ->
+    Tl_bisim (tl eta S c) (tl eta S' c') ->
+    R_trace_bisim_equivalence' S S'.
+Hint Constructors R_trace_bisim_equivalence' : tleq.
 
 
-Theorem trace_equality_equivalence :
-  forall S S' eta
-  (Swf : wellformed S)
-  (S'wf : wellformed S'),
-  tl eta S (wellformed_Contractive S Swf) =
-    tl eta S' (wellformed_Contractive S' S'wf) ->
+Lemma trace_bisim_equivalence' :
+  forall S S' eta c c',
+  wellformed S ->
+  wellformed S' ->
+  Tl_bisim (tl eta S c) (tl eta S' c') ->
   sequiv S S'.
 Proof.
-  Ltac solve_different_shape H := simpl in H; discriminate H.
+  Ltac solve_same_shape H :=
+    inverts2 H; constructor; econstructor; eauto with wf
+  .
 
-  Ltac solve_wellformed_var H :=
+  Ltac solve_mu H :=
+    erewrite tl_mu_subst in H; [constructor; econstructor|]; eauto with free wf
+  .
+
+  Ltac solve_wellformed_var :=
     match goal with
-    | _ : wellformed (var _) |- _ =>
-      clear H; eauto with wf
+    | _ : wellformed (var _) |- _ => auto with wf
     end
   .
 
-  Ltac solve_mu H := erewrite tl_mu_subst in H; eauto with tleq free.
-
-  Ltac solve_same_shape H :=
-    inverts2 H; constructor; econstructor;
-      match goal with
-      | |- tl _ ?s _ = tl _ ?s' _ =>
-        erewrite tl_contractive_irrelevant with (S := s);
-        erewrite tl_contractive_irrelevant with (S := s')
-      end;
-      eassumption
-  .
-
-  introv H. apply sequiv_coind with (R := R_trace_equality_equivalence);
+  intros. apply sequiv_coind with (R := R_trace_bisim_equivalence');
     [|econstructor; eauto].
-  clear. introv HR. inverts HR. rename H into Heq. destruct S; destruct S';
-    solve
+  clear. introv H. inverts H. rename H2 into Heq. destruct S; destruct S';
+    try solve
       [ constructor
-      | solve_wellformed_var Heq
-      | solve_different_shape Heq
+      | solve_wellformed_var
       | solve_mu Heq
       | solve_same_shape Heq
       ].
 Unshelve.
-  all:
-    repeat match goal with
-    | H : tl _ _ _ = tl _ _ _ |- _ =>
-        clear H
-    end;
-    eauto with subst wf.
+  all: eauto with contractive subst.
 Qed.
-
-
-Inductive R_trace_bisim_equivalence : Sty -> Sty -> Prop :=
-| R_trace_bisim_equivalence_intro :
-    forall S S' eta (Swf : wellformed S) (S'wf : wellformed S'),
-    Tl_bisim (tl eta S (wellformed_Contractive S Swf))
-      (tl eta S' (wellformed_Contractive S' S'wf)) ->
-    R_trace_bisim_equivalence S S'.
-Hint Constructors R_trace_bisim_equivalence : tleq.
-
 
 Theorem trace_bisim_equivalence :
   forall S S' eta
   (Swf : wellformed S)
-  (S'wf : wellformed S'),
-  Tl_bisim (tl eta S (wellformed_Contractive S Swf))
-    (tl eta S' (wellformed_Contractive S' S'wf)) ->
+  (Swf' : wellformed S'),
+  Tl_bisim
+    (tl eta S (wellformed_Contractive Swf))
+    (tl eta S' (wellformed_Contractive Swf')) ->
+  sequiv S S'.
+Proof. intros. eapply trace_bisim_equivalence'; eauto. Qed.
+
+Theorem trace_eq_equivalence :
+  forall S S' eta
+  (Swf : wellformed S)
+  (Swf' : wellformed S'),
+  (tl eta S (wellformed_Contractive Swf)) =
+    (tl eta S' (wellformed_Contractive Swf')) ->
   sequiv S S'.
 Proof.
-  Ltac solve_same_shape' H :=
-    inverts2 H; constructor; econstructor;
-    match goal with
-    | |- Tl_bisim (tl _ ?s _) (tl _ ?s' _) =>
-      erewrite tl_contractive_irrelevant with (S := s);
-      erewrite tl_contractive_irrelevant with (S := s')
-    end;
-    eassumption
-  .
-
-  introv H. apply sequiv_coind with (R := R_trace_bisim_equivalence);
-    [|econstructor; eauto].
-  clear. introv H. inverts1 H. rename H into Heq. destruct S; destruct S';
-    try solve
-    [ constructor
-    | solve_wellformed_var Heq
-    | inverts2 Heq
-    | solve_mu Heq
-    | solve_same_shape' Heq
-    ].
-Unshelve.
-  all:
-    repeat match goal with
-    | H : Tl_bisim (tl _ _ _) (tl _ _ _) |- _ =>
-        clear H
-    end;
-    eauto with wf subst.
-Qed.
+  introv Heq. eapply trace_bisim_equivalence. rewrite Heq. Abort.
 
 
 Inductive R_equivalence_trace_bisim' : Tl -> Tl -> Prop :=
@@ -120,7 +80,8 @@ Inductive R_equivalence_trace_bisim' : Tl -> Tl -> Prop :=
      wellformed S' /\
      sequiv (cs S) (cs S')
     ) ->
-    R_equivalence_trace_bisim' l l'.
+    R_equivalence_trace_bisim' l l'
+.
 
 
 (* TODO ouch *)
@@ -131,89 +92,91 @@ Lemma equivalence_trace_bisim' :
   sequiv S S' ->
   Tl_bisim (tl eta S c) (tl eta S' c').
 Proof.
+  Ltac wf_inv S1 H1 S2 :=
+    let Htmp := fresh in
+    assert (wellformed S1) as Htmp by (rewrite H1; auto with wf);
+    assert (wellformed S2) by (auto with wf);
+    clear Htmp
+  .
+
   intros. (rewrite_strat (subterms cs_preserves_tl)); try assumption.
   apply Tl_bisim_coind with (R := R_equivalence_trace_bisim').
   - clear. introv CIH. inverts1 CIH. norm_hyp_auto.
     rename H0 into Hwf. rename H2 into Hwf'. rename H4 into Hsequiv.
     subst. inverts2 Hsequiv.
     * gen c c' Hwf Hwf'. rewrite <- Hsequiv. rewrite <- H2.
-      clear Hsequiv. clear H2.
-      introv Hwf Hwf'. constructor.
+      clear Hsequiv. intros. constructor.
     * gen c c' Hwf Hwf'. rewrite <- H0. rewrite <- H1.
       introv Hwf Hwf'.
-      assert (wellformed (send B S0)) as Htmp1 by (rewrite H0; auto with subst).
-      assert (wellformed (send B S'0)) as Htmp2 by (rewrite H1; auto with subst).
-      apply wellformed_inv in Htmp1. apply wellformed_inv in Htmp2.
+      wf_inv (send B S0) H0 S0.
+      wf_inv (send B S'0) H1 S'0.
       simpl. constructor. econstructor.
       exists S0 S'0. eexists. eexists. splits.
       + symmetry. apply cs_preserves_tl. assumption.
       + symmetry. apply cs_preserves_tl. assumption.
       + assumption.
       + assumption.
-      + apply cs_preserves_sequiv; eauto.
+      + apply cs_preserves_sequiv; eauto with wf.
     * gen c c' Hwf Hwf'. rewrite <- H0. rewrite <- H1.
       introv Hwf Hwf'.
-      assert (wellformed (recv B S0)) as Htmp1 by (rewrite H0; auto with subst).
-      assert (wellformed (recv B S'0)) as Htmp2 by (rewrite H1; auto with subst).
-      apply wellformed_inv in Htmp1. apply wellformed_inv in Htmp2.
+      wf_inv (recv B S0) H0 S0.
+      wf_inv (recv B S'0) H1 S'0.
       simpl. constructor. econstructor.
       exists S0 S'0. eexists. eexists. splits.
       + symmetry. apply cs_preserves_tl. assumption.
       + symmetry. apply cs_preserves_tl. assumption.
       + assumption.
       + assumption.
-      + apply cs_preserves_sequiv; eauto.
+      + apply cs_preserves_sequiv; eauto with wf.
     * gen c c' Hwf Hwf'. rewrite <- H0. rewrite <- H1.
       introv Hwf Hwf'.
-      assert (wellformed (echoice S1 S2)) as Htmp1 by (rewrite H0; auto with subst).
-      assert (wellformed (echoice S1' S2')) as Htmp2 by (rewrite H1; auto with subst).
-      apply wellformed_inv in Htmp1. apply wellformed_inv in Htmp2.
-      destruct Htmp1. destruct Htmp2.
+      wf_inv (echoice S1 S2) H0 S1.
+      wf_inv (echoice S1 S2) H0 S2.
+      wf_inv (echoice S1' S2') H1 S1'.
+      wf_inv (echoice S1' S2') H1 S2'.
       simpl. constructor.
       + econstructor. exists S1. exists S1'. eexists. eexists. splits.
         -- symmetry. apply cs_preserves_tl. assumption.
         -- symmetry. apply cs_preserves_tl. assumption.
         -- assumption.
         -- assumption.
-        -- apply cs_preserves_sequiv; eauto.
+        -- apply cs_preserves_sequiv; eauto with wf.
       + econstructor. exists S2. exists S2'. eexists. eexists. splits.
         -- symmetry. apply cs_preserves_tl. assumption.
         -- symmetry. apply cs_preserves_tl. assumption.
         -- assumption.
         -- assumption.
-        -- apply cs_preserves_sequiv; eauto.
+        -- apply cs_preserves_sequiv; eauto with wf.
     * gen c c' Hwf Hwf'. rewrite <- H0. rewrite <- H1.
       introv Hwf Hwf'.
-      assert (wellformed (ichoice S1 S2)) as Htmp1 by (rewrite H0; auto with subst).
-      assert (wellformed (ichoice S1' S2')) as Htmp2 by (rewrite H1; auto with subst).
-      apply wellformed_inv in Htmp1. apply wellformed_inv in Htmp2.
-      destruct Htmp1. destruct Htmp2.
+      wf_inv (ichoice S1 S2) H0 S1.
+      wf_inv (ichoice S1 S2) H0 S2.
+      wf_inv (ichoice S1' S2') H1 S1'.
+      wf_inv (ichoice S1' S2') H1 S2'.
       simpl. constructor.
       + econstructor. exists S1. exists S1'. eexists. eexists. splits.
         -- symmetry. apply cs_preserves_tl. assumption.
         -- symmetry. apply cs_preserves_tl. assumption.
         -- assumption.
         -- assumption.
-        -- apply cs_preserves_sequiv; eauto.
+        -- apply cs_preserves_sequiv; eauto with wf.
       + econstructor. exists S2. exists S2'. eexists. eexists. splits.
         -- symmetry. apply cs_preserves_tl. assumption.
         -- symmetry. apply cs_preserves_tl. assumption.
         -- assumption.
         -- assumption.
-        -- apply cs_preserves_sequiv; eauto.
+        -- apply cs_preserves_sequiv; eauto with wf.
     * symmetry in H0. apply cs_mu_absurd in H0.
       + contradiction.
-      + eauto with wf.
+      + eauto with contractive wf.
     * symmetry in H0. apply cs_mu_absurd in H0.
       + contradiction.
-      + eauto with wf.
+      + eauto with contractive wf.
   - econstructor. exists S. exists S'. eexists. eexists. splits;
     auto with subst.
-    * apply cs_preserves_sequiv; eauto with wf.
+    * apply cs_preserves_sequiv; assumption.
 Unshelve.
-  all:
-    try solve
-      [apply wellformed_Contractive; auto with subst].
+  all: auto with wf.
 Qed.
 
 Theorem equivalence_trace_bisim :
@@ -221,6 +184,6 @@ Theorem equivalence_trace_bisim :
   (Swf : wellformed S)
   (S'wf : wellformed S'),
   sequiv S S' ->
-  Tl_bisim (tl eta S (wellformed_Contractive _ Swf))
-    (tl eta S' (wellformed_Contractive _ S'wf)).
+  Tl_bisim (tl eta S (wellformed_Contractive Swf))
+    (tl eta S' (wellformed_Contractive S'wf)).
 Proof. intros. apply equivalence_trace_bisim'; auto. Qed.
