src/Transitivity.v
@@ -1,4 +1,5 @@
-Require Import CS CSFacts Equiv Reflexivity Sty StyInd Subst SubstFacts Tac Wf.
+Require Import CS CSFacts Equiv Reflexivity Sty StyInd Subst SubstFacts Tac Wf
+  WfFacts.
 
 Create HintDb trans discriminated.
 Hint Resolve sequiv_reflexive : trans.
@@ -55,11 +56,11 @@ Theorem sequiv_transitive :
 Proof.
   apply trans_helper_transitive. apply sequiv_coind.
   introv H. rename S' into U. inverts H.
-  assert (sequiv S (cs T)) as HSeqT by (
-    eapply cs_preserves_sequiv_r; eauto with subst
+  assert (sequiv S (cs T)) as HSeqT  by (
+    eapply cs_preserves_sequiv_r; eauto with wf
   ).
   assert (sequiv (cs T) U) as HTeqU by (
-    eapply cs_preserves_sequiv_l; eauto with subst
+    eapply cs_preserves_sequiv_l; eauto with wf
   ).
   clear H3 H4. inverts2 HSeqT; inverts2 HTeqU; subst; try solve [false].
 
@@ -72,84 +73,81 @@ Proof.
   (* send *)
   - rewrite <- H4 in H3. injection H3; intros; subst.
     constructor. apply trans_helper_trans with (T := S); eauto with wf.
-      apply cs_preserves_wellformedness in H1. rewrite <- H4 in H1.
+      apply cs_preserves_wellformed in H1. rewrite <- H4 in H1.
       eauto with wf.
 
   - constructor. rewrite <- H3 in *.
     apply trans_helper_trans with (T := send B S'); eauto with wf.
-      rewrite H3. eapply cs_preserves_wellformedness; eauto with wf.
+      rewrite H3. eauto with wf.
 
   (* recv *)
   - rewrite <- H4 in H3. injection H3; intros; subst.
     constructor. apply trans_helper_trans with (T := S); eauto with wf.
-      apply cs_preserves_wellformedness in H1. rewrite <- H4 in H1.
+      apply cs_preserves_wellformed in H1. rewrite <- H4 in H1.
       eauto with wf.
 
   - constructor. rewrite <- H3 in *.
     apply trans_helper_trans with (T := recv B S'); eauto with wf.
-      rewrite H3. eapply cs_preserves_wellformedness; eauto with wf.
+      rewrite H3. eauto with wf.
 
   (* echoice *)
-  - assert (wellformed (echoice S1' S2')) by
-      (rewrite H3; eapply cs_preserves_wellformedness; eauto with wf).
+  - assert (wellformed (echoice S1' S2')) by (rewrite H3; eauto with wf).
     rewrite <- H4 in H3. injection H3; intros; subst.
     constructor.
     * apply trans_helper_trans with (T := S0); eauto with wf.
     * apply trans_helper_trans with (T := S3); eauto with wf.
 
-  - assert (wellformed (echoice S1' S2')) by
-      (rewrite H3; eapply cs_preserves_wellformedness; eauto with wf).
+  - assert (wellformed (echoice S1' S2')) by (rewrite H3; eauto with wf).
     constructor. rewrite <- H3 in *.
     apply trans_helper_trans with (T := echoice S1' S2'); eauto with wf.
 
   (* ichoice *)
-  - assert (wellformed (ichoice S1' S2')) by
-      (rewrite H3; eapply cs_preserves_wellformedness; eauto with wf).
+  - assert (wellformed (ichoice S1' S2')) by (rewrite H3; eauto with wf).
     rewrite <- H4 in H3. injection H3; intros; subst.
     constructor.
     * apply trans_helper_trans with (T := S0); eauto with wf.
     * apply trans_helper_trans with (T := S3); eauto with wf.
 
-  - assert (wellformed (ichoice S1' S2')) by
-      (rewrite H3; eapply cs_preserves_wellformedness; eauto with wf).
+  - assert (wellformed (ichoice S1' S2')) by (rewrite H3; eauto with wf).
     constructor. rewrite <- H3 in *.
     apply trans_helper_trans with (T := ichoice S1' S2'); eauto with wf.
 
   (* unit *)
-  - rewrite <- HTeqU in *. constructor. apply sequiv_impl_trans_helper; auto with wf.
+  - rewrite <- HTeqU in *. constructor. apply sequiv_impl_trans_helper;
+      auto with wf.
 
   (* send *)
   - constructor. rewrite <- H3 in *.
     apply trans_helper_trans with (T := send B S); auto with wf.
-      rewrite H3; eauto using cs_preserves_wellformedness with wf.
+      rewrite H3; eauto with wf.
 
   (* recv *)
   - constructor. rewrite <- H3 in *.
     apply trans_helper_trans with (T := recv B S); auto with wf.
-      rewrite H3; eauto using cs_preserves_wellformedness with wf.
+      rewrite H3; eauto with wf.
 
   (* echoice *)
   - constructor. rewrite <- H3 in *.
     apply trans_helper_trans with (T := echoice S1 S2); auto with wf.
-      rewrite H3; eauto using cs_preserves_wellformedness with wf.
+      rewrite H3; eauto with wf.
 
   (* ichoice *)
   - constructor. rewrite <- H3 in *.
     apply trans_helper_trans with (T := ichoice S1 S2); auto with wf.
-      rewrite H3; eauto using cs_preserves_wellformedness with wf.
+      rewrite H3; eauto with wf.
 
   (* mu 1 (impossible) *)
-  - exfalso; eauto using cs_mu_absurd.
+  - exfalso; eauto with subst wf.
 
   (* mu 2 *)
   - constructor.
     assert (sequiv (cs T) (mu X0 S')) as HTeqU' by auto.
     apply trans_helper_trans with (T := cs T);
-      eauto using cs_preserves_wellformedness with wf.
+      eauto with wf.
 
   (* mu 3 (impossible) *)
-  - exfalso; eauto using cs_mu_absurd.
+  - exfalso; eauto with subst wf.
 
   (* mu 4 (impossible) *)
-  - exfalso; eauto using cs_mu_absurd.
+  - exfalso; eauto with subst wf.
 Qed.
