src/WfFacts.v
@@ -1,0 +1,35 @@
+Require Import Contractive ContractiveFacts CSFacts Free FreeFacts SubstFacts
+  Sty Tac Wf.
+
+
+Hint Resolve cs_preserves_wellformed : wf.
+Hint Resolve wellformed_Contractive : wf.
+Hint Resolve wellformed_Closed : wf.
+Hint Resolve mu_unfold_preserves_wellformed : wf.
+
+
+Lemma wellformed_inv :
+  (forall B S, wellformed (send B S) -> wellformed S) /\
+  (forall B S, wellformed (recv B S) -> wellformed S) /\
+  (forall S1 S2, wellformed (echoice S1 S2) -> wellformed S1 /\ wellformed S2) /\
+  (forall S1 S2, wellformed (ichoice S1 S2) -> wellformed S1 /\ wellformed S2).
+Proof. splits; unfold wellformed; auto with contractive free. Qed.
+
+
+Hint Extern 2 (wellformed _) =>
+  match goal with
+  | H : wellformed _ |- _ =>
+      solve [apply wellformed_inv in H; try (decompose_and H); assumption]
+  end
+: wf.
+
+
+Hint Extern 2 =>
+  match goal with
+  | H : wellformed (var _) |- _ =>
+      solve [
+        unfold wellformed in H; destruct H as [_ H]; apply Closed_var_absurd in H;
+        contradiction
+      ]
+  end
+: wf.
